clean up a bit + generic thms + example disc

theories/logrel/definition.v
@@ -111,10 +111,18 @@ Definition open_exprel_typed (Γ : list type) (L : LabelRel) (e e' : expr) (τ :
       big_sepL3 (fun τ v v' => valrel_typed τ Δ v v') Γ vs vs' ⊢
           exprel_typed τ Δ e.[subst_list (of_val <$> vs)] e'.[subst_list (of_val <$> vs')].
 
-Lemma open_exprel_typed_weaken (L L' : LabelRel) (H : L ⊑ L')
-  (Γ : list type) (e e' : expr) (τ : type) :
-  open_exprel_typed Γ L e e' τ → open_exprel_typed Γ L' e e' τ.
-Proof. intros. intros Δ HL'Δ. apply H0. by eapply le_permissive_trans'. Qed.
+Definition sem_typed_liable_to (L : label → Prop) Γ (e : expr) τ : Prop :=
+    open_exprel_typed Γ (diagonal L) e e τ ∧ Closed_n (length Γ) e.
+
+Notation sem_typed := (sem_typed_liable_to (fun _ => False)).
+
+(* Definition sem_typed Γ e τ : Prop := open_exprel_typed Γ ⊥ e e τ. *)
+
+Lemma open_exprel_typed_weaken {L L' : LabelRel} {Γ e e' τ} :
+  open_exprel_typed Γ L e e' τ →
+  L ⊑ L' →
+  open_exprel_typed Γ L' e e' τ.
+Proof. intros. intros Δ HL'Δ. apply H. by eapply le_permissive_trans'. Qed.
 
 Lemma open_exprel_typed_app_ctx Γ' (L : LabelRel)
   (Γ : list type) (e e' : expr) (He : Closed_n (length Γ) e) (He' : Closed_n (length Γ) e') (τ : type) :
@@ -144,6 +152,18 @@ Lemma ctx_rel_typed_weaken C C' (L L' : LabelRel) (H : le_permissive L L')
   ctx_rel_typed L C C' Γ1 τ1 Γ2 τ2 → ctx_rel_typed L' C C' Γ1 τ1 Γ2 τ2.
 Proof.
   intros. intros Δ HL'Δ e e' Hee'. apply H0; auto. eapply le_permissive_trans_inst; eauto. Qed.
+
+Lemma rel_ctx_fill_expr {L Le Lc : LabelRel} {Γ τ Γ' τ' e e' C C'}
+    {Hee' : open_exprel_typed Γ Le e e' τ}
+    {HCC' : ctx_rel_typed Lc C C' Γ τ Γ' τ'}
+    (H : Le ⊔ Lc ⊑ L) :
+  open_exprel_typed Γ' L (fill_ctx C e) (fill_ctx C' e') τ'.
+Proof.
+  eapply open_exprel_typed_weaken.
+  apply (HCC' (Le ⊔ Lc)). by apply le_permissive_join_r.
+  eapply open_exprel_typed_weaken. apply Hee'.
+  by apply le_permissive_join_l. auto.
+Qed.
 
 (* Lemma open_exprel_typed_compose L12 L23 Γ1 Γ2 Γ3 C12 C12' C23 C23' τ1 τ2 τ3 : *)
 (*   ctx_rel_typed L12 C12 C12' Γ1 τ1 Γ2 τ2 → *)
