theories/logrel/examples/main.v
@@ -8,12 +8,9 @@ From iris.si_logic Require Export bi.
 From iris.proofmode Require Import tactics.
 (* From iris.proofmode Require Import base proofmode classes. *)
 
-
 Section examples.
 
   Context {ν : label} {Hν : NeverOccurs ν}.
-
-  Definition sem_typed Γ e τ : Prop := open_exprel_typed Γ ⊥ e e τ.
 
   Definition example1 : expr :=
     Lam (
@@ -25,6 +22,7 @@ Section examples.
   Lemma example1_sem_typed :
     sem_typed [] example1 (Bin Arrow (Base Int) (Base Int)).
   Proof.
+    split; [| by intros σ; asimpl ].
     iIntros (Δ HΔ vs vs') "_". asimpl. rfn_val.
     iIntros (w w') "Hww'". dvals w w'. iRewrite "Hww'". simpl.
     rfn_steps. rewrite bool_decide_true; try by lia. rfn_val.
@@ -46,12 +44,14 @@ Section examples.
          )
       ).
 
+
   Lemma example2_sem_typed :
     sem_typed [] example2 (Bin Arrow (Bin Arrow (Base Int) (Base Int)) (Base Int)).
   Proof.
+    split; [| by intros σ; asimpl ].
     iIntros (Δ HΔ vs vs') "_". rfn_steps. rfn_val. iNext.
     iIntros (h h') "#Hhh'". dvals h h'. simpl. rfn_steps.
-    rfn_bind'. rw_of_val. iApply "Hhh'". auto. iNext.
+    rfn_bind. rw_of_val. iApply "Hhh'". auto. iNext.
     iIntros (v v') "Hvv'". dvals v v'. iRewrite "Hvv'".
     rfn_steps. rfn_val.
   Qed.
@@ -63,6 +63,7 @@ Section examples.
     sem_typed [] example3 (Bin Arrow (Bin Sum (Base Unit) (Base Bool))
                              (Bin Sum (Base Unit) (Base Unit))).
   Proof.
+    split; [| by intros σ; asimpl ].
     iIntros (Δ HΔ vs vs') "_". asimpl. rfn_val.
     iIntros (s s') "#Hss'". dvals s s'; rfn_steps; rfn_val.
   Qed.
