theories/maps/linker/components/agree.v
@@ -1,5 +1,5 @@
 From main.prelude Require Import imports autosubst base_lang lists labels.
-From main.grad_lang Require Import types.
+From main.grad_lang Require Import definition types.
 From main.dyn_lang Require Import definition contexts lib casts.
 From main.maps Require Import grad_into_dyn.definition.
 From main.maps.linker.components Require Import dyn grd.
@@ -8,14 +8,14 @@ Section agree.
 
   Context {ν : label} {Hν : NeverOccurs ν}.
 
-  Lemma LamN_agree n e : ⌊ grd.LamN n e ⌋ = dyn.LamN n ⌊ e ⌋.
+  Lemma LamN_agree n e : ⟨ grd.LamN n e ⟩ = dyn.LamN n ⟨ e ⟩.
   Proof. induction n; auto. simpl. by rewrite IHn. Qed.
 
   Lemma LamN_ctx_agree n : trns_ctx $ grd.LamN_ctx n = dyn.LamN_ctx n.
   Proof. induction n; auto. simpl. by rewrite IHn. Qed.
 
   Lemma AppWithList_agree e fs :
-    ⌊ grd.AppWithList e fs ⌋ = dyn.AppWithList ⌊ e ⌋ ((fun f => ⌊ f ⌋) <$> fs).
+    ⟨ grd.AppWithList e fs ⟩ = dyn.AppWithList ⟨ e ⟩ ((fun f => ⟨ f ⟩) <$> fs).
   Proof.
     induction fs as [|f fs']; first auto.
     rewrite /= /AppAn. f_equiv. by rewrite /IHfs'.
@@ -29,11 +29,11 @@ Section agree.
   Qed.
 
   Lemma wrap_ctx_vars_ascribe_up_agree (ℓ : label) (Γ : list type) :
-    trns <$> (grd.wrap_ctx_vars_ascribe_up ℓ Γ) = dyn.wrap_ctx_vars_ascribe_up ℓ Γ.
+    trns <$> (grd.WrapVars ((fun τ => Ascribe ℓ τ Unknown) <$> Γ)) = dyn.WrapVars ((fun τ => App ν (of_val $ cast' ℓ τ Unknown)) <$> Γ).
   Proof.
-    rewrite /grd.wrap_ctx_vars_ascribe_up /dyn.wrap_ctx_vars_ascribe_up.
-    rewrite fmap_imap. apply imap_ext. intros. simpl. rewrite /cast'.
-    destruct (consistency_decision x Unknown); auto.
+    rewrite /grd.WrapVars /dyn.WrapVars.
+    rewrite fmap_imap. repeat rewrite imap_fmap. apply imap_ext.
+    intros. by simpl.
   Qed.
 
 End agree.
