theories/maps/linker/components/lemmas.v
@@ -1,22 +1,68 @@
-From main.prelude Require Import imports autosubst base_lang lists labels.
-From main.grad_lang Require Import types typing labels.
-From main.dyn_lang Require Import definition contexts lib casts.
-From main.maps.linker.components Require Import grd common agree dyn.
-
-
-
-From main.prelude Require Import big_op_three.
-From main.dyn_lang Require Import lemmas tactics.
+From main.grad_lang Require Import types labels.
+From main.dyn_lang Require Import definition casts lib tactics lemmas.
 From main.logrel Require Import rfn definition lib.small_helpers lemmas.casts_superfluous lemmas.fun_grad_into_dyn.
-From iris.si_logic Require Export bi.
+From main.maps.linker.components Require Import common grd dyn agree.
+
+From main.prelude Require Import big_op_three labels autosubst.
 From iris.proofmode Require Import tactics.
 
 Section superfluous_l.
 
+  (* wanna avoid proving termination *)
+
   Context {ν : label} {Hν : NeverOccurs ν}.
 
-  Lemma LamN_ctx_no_lables n : InGradCtx (grd.LamN_ctx n) ⊑ ⊥.
-  Proof. rewrite /InGradCtx /diagonal; intros l l'. induction n; set_solver. Qed.
+  Lemma open_exprel_superfluous_rtn_l L ℓ Γ e e' τ :
+    open_exprel_typed Γ L e e' τ →
+    open_exprel_typed Γ L
+      (App ν (of_val $ cast' ℓ Unknown τ) e) e' τ.
+  Proof.
+    iIntros (Hee' Δ HLΔ vs vs') "#Hvsvs'". rewrite /= cast'_closed.
+    rw_fill.
+    iApply (@rfn_bindK [AppRCtx _ _] []). eauto. eauto. iApply Hee'; eauto.
+    simpl.
+    iApply cast_upwards_val_superfluous_l.
+  Qed.
+
+  Lemma open_exprel_superfluous_ctx_l_help ℓ α L (Γ : list type) :
+    ⊢ ∀ Λ Λ' vs vs', big_sepL3 (fun τ v v' => valrel_typed τ L v v') Γ vs vs' -∗
+        exprel_typed (LamN_type Γ α) L Λ Λ' -∗
+          exprel_typed α L
+            (AppWithList Λ (zip_with (λ τ0 e0, App ν (of_val (cast' ℓ τ0 Unknown)) e0) Γ (of_val <$> vs)))
+            (AppWithList Λ' (zip_with (λ τ0 e0, App ν (of_val (LamV (Var 0))) e0) Γ (of_val <$> vs'))).
+  Proof.
+    induction Γ as [|τ Γn IHΓ] using rev_ind; try by auto.
+    iIntros (Λ Λ' vs vs') "#Hvsvs'".
+    (* pure admin to get lists of right shape etc.. *)
+    iDestruct (big_sepL3_length with "Hvsvs'") as "[%eq1 %eq2]".
+    rewrite -eq1 in eq2. rewrite app_length Nat.add_1_r in eq1, eq2.
+    destruct vs as [| v vsn] using rev_ind; try by inversion eq1. clear IHvsn.
+    destruct vs' as [| v' vsn'] using rev_ind; try by inversion eq2. clear IHvsn'.
+    iDestruct (big_sepL3_app_inv with "Hvsvs'") as "[#Hvsvs'' [#Hvv' _]]"; auto.
+    repeat rewrite app_length Nat.add_1_r in eq1, eq2. inversion eq1. inversion eq2. clear eq1 eq2.
+    iIntros "#HΛΛ'".
+    (* make it to values *)
+    rewrite LamN_type_snoc. do 2 rewrite AppWithList_ectx_agree'.
+    rfn_bind. iApply "HΛΛ'". iClear "HΛΛ'". clear Λ Λ'. iIntros (Λ Λ') "#HΛΛ'".
+    (* some more rewriting *)
+    do 2 rewrite fmap_app.
+    do 2 (rewrite zip_with_app; [|by rewrite fmap_length]). simpl.
+    rewrite /AppWithList_ectx. do 2 rewrite fmap_app. do 2 rewrite fill_app.
+    change (AppLCtx ν <$> zip_with ?f ?a ?b) with (@AppWithList_ectx ν (zip_with f a b)). simpl.
+    rw_fill_popped. do 4 rewrite -(fill_app).
+    rfn_bind. rfn_steps.
+    { rewrite cast_upwards_rw. change (App ν) with (AppAn).
+      iApply (cast_upwards_val_superfluous_l ℓ τ L $! Normal with "Hvv'"). }
+    iIntros (w w') "#Hww'".
+    (* prepare to use HΛΛ' *)
+    do 2 rewrite app_nil_r.
+    do 2 rewrite fill_app. simpl. dvals Λ Λ'.
+    rfn_bind. rfn_steps. by iApply "HΛΛ'". iClear "Hww' HΛΛ'".
+    (* use IH *)
+    iIntros (Λ Λ') "HΛΛ'".
+    do 2 rewrite -(AppWithList_ectx_agree').
+    iApply IHΓ; eauto. rfn_val.
+  Qed.
 
   Lemma LamN_ctx_rel_typed Γ τ :
     ctx_rel_typed ⊥ (LamN_ctx (length Γ)) (LamN_ctx (length Γ)) Γ τ [] (LamN_type Γ τ).
@@ -30,22 +76,23 @@ Section superfluous_l.
   Lemma open_exprel_LamN_type Γ L e e' τ :
     open_exprel_typed Γ L e e' τ →
     open_exprel_typed [] L
-      (LamN (length Γ) e)
-      (LamN (length Γ) e') (LamN_type Γ τ).
+    (LamN (length Γ) e)
+    (LamN (length Γ) e') (LamN_type Γ τ).
   Proof. intro Hee'. do 2 rewrite -fill_LamN_ctx. apply LamN_ctx_rel_typed. intros ℓ ℓ' Hll. exfalso. apply Hll. auto. Qed.
+
 
   Lemma open_exprel_superfluous_ctx_l  L ℓ Γ e (HCe : Closed_n (length Γ) e) e' τ :
     open_exprel_typed Γ L e e' τ →
     open_exprel_typed Γ L
       (AppWithList (LamN (length Γ) ((App ν (of_val $ cast' ℓ Unknown τ) e)))
-                   (wrap_ctx_vars_ascribe_up ℓ Γ))
+                   (WrapVars ((fun τ => App ν (of_val $ cast' ℓ τ Unknown)) <$> Γ)))
       e' τ.
   Proof.
     intros Hee'.
     iIntros (Δ HLΔ vs vs') "#Hvsvs'".
     iDestruct (big_sepL3_length with "Hvsvs'") as "[%eq1 %eq2]". rewrite -eq1 in eq2.
     iApply (rfn_steps_r_inv (AppWithList (LamN _ e') (zip_with (λ τ0 e0, AppAn (of_val (LamV (Var 0))) e0) Γ (of_val <$> vs')))).
-    { eapply LamN_AppWithList_rtc_to_vals.
+    { eapply LamN_AppWithList_to_vals.
       rewrite zip_with_fmap_r.
       assert (zip_with
        (λ (_ : type) (z : val),
@@ -61,17 +108,108 @@ Section superfluous_l.
       apply Forall2_fmap_l. apply Forall_Forall2_diag. simpl.
       apply Forall_true. intros. apply rtc_once. step_solver. }
     rewrite AppWithList_subst.
-    rewrite wrap_ctx_vars_ascribe_up_subst.
+    rewrite WrapVars_subst.
     rewrite LamN_subst. change (App ν ?a ?b).[?σ] with (App ν a.[σ] b.[σ]). rewrite HCe /= cast'_closed.
+    rewrite zip_with_fmap_l.
     iApply (open_exprel_superfluous_ctx_l_help ℓ τ Δ Γ with "Hvsvs'").
     rewrite zip_with_length_l.
     assert (Hee'' := (open_exprel_superfluous_rtn_l _ ℓ _ _ _ _ Hee')).
     assert (Hee''' := open_exprel_LamN_type Γ L _ _ τ Hee'').
     specialize (Hee''' Δ HLΔ [] []). asimpl in Hee'''.
     rewrite -cast_downwards_rw in Hee'''. iApply Hee'''. eauto.
-    rewrite fmap_length. lia.
-    rewrite fmap_length. lia.
+    rewrite fmap_length. lia. apply Forall_fmap, Forall_true.
+    intros t σ. asimpl. by rewrite cast'_closed.
+    repeat rewrite fmap_length. lia.
   Qed.
 
-
 End superfluous_l.
+
+From main.logrel Require Import lib.weakestpre.
+
+Section superfluous_r.
+
+  Context {ν : label} {Hν : NeverOccurs ν}.
+
+  Lemma open_exprel_superfluous_rtn_r L ℓ Γ e e' τ :
+    open_exprel_typed Γ L e e' τ →
+    open_exprel_typed Γ L
+      e (App ν (of_val $ cast' ℓ Unknown τ) e') τ.
+  Proof.
+    iIntros (Hee' Δ HLΔ vs vs') "#Hvsvs'". rewrite /= cast'_closed.
+    rw_fill.
+    iApply (@rfn_bindK [] [AppRCtx _ _]). eauto. eauto. iApply Hee'; eauto.
+    simpl.
+    iApply cast_upwards_val_superfluous_r.
+  Qed.
+
+  Lemma help_r Δ ℓ Γ vs vs' :
+    ⊢ big_sepL3
+        (λ (τ : type) (v v' : val), valrel_typed τ Δ v v') Γ vs vs' -∗
+    ∃ (ws' : list val),
+      big_sepL3
+        (λ (τ : type) (v w' : val), valrel_typed τ Δ v w') Γ vs ws' ∗
+      ⌜ Forall3 (λ (τ : type) (v' w' : val), rtc step_ne (App ν (of_val $ cast' ℓ τ Unknown) (of_val v')) (of_val w') ) Γ vs' ws' ⌝.
+  Proof.
+    revert vs vs'.
+    iInduction Γ as [|τ  Γ] "IH".
+    - iIntros (vs vs') "Hvsvs'"; destruct vs as [|v vs]; auto; destruct vs' as [|v' vs']; auto; simpl. iExists []. iSplit; auto. iPureIntro. constructor.
+    - iIntros (vs vs') "Hvsvs'"; destruct vs as [|v vs]; destruct vs' as [|v' vs']; auto.
+      simpl. iDestruct "Hvsvs'" as "[Hvv' Hvsvs']". iSpecialize ("IH" with "Hvsvs'").
+      iDestruct "IH" as (ws') "[H1 %H2]".
+      (* use superfluous lemma *)
+      iDestruct (cast_upwards_val_superfluous_r ℓ τ Δ $! Normal with "Hvv'") as "HHH".
+      iDestruct (wp_val_inv with "HHH") as "HHH'".
+      iDestruct "HHH'" as (w') "[%Hs Hvw']".
+      iExists (w' :: ws'). iFrame. iPureIntro. constructor. by rewrite cast_upwards_rw. auto.
+  Qed.
+
+  Lemma open_exprel_superfluous_ctx_r_help L ℓ Γ e e' (He' : Closed_n (length Γ) e') τ :
+    open_exprel_typed Γ L e e' τ →
+    open_exprel_typed Γ L
+      e
+      (AppWithList (LamN (length Γ) e')
+                   (WrapVars ((fun τ => App ν (of_val $ cast' ℓ τ Unknown)) <$> Γ))) τ.
+  Proof.
+    intros Hee'.
+    iIntros (Δ HLΔ vs vs') "#Hvsvs'".
+    iDestruct (big_sepL3_length with "Hvsvs'") as "[%eq1 %eq2]". rewrite -eq1 in eq2.
+    iDestruct (help_r Δ ℓ with "Hvsvs'") as (ws') "[Hvs'ws' %Hs]".
+    assert (eq3 := Forall3_length_lr _ _ _ _ Hs).
+    iApply (rfn_steps_r e'.[subst_list (of_val <$> ws')]).
+    { rewrite AppWithList_subst LamN_subst.
+      rewrite WrapVars_subst.
+      rewrite zip_with_fmap_r.
+      repeat rewrite /= He'.
+      assert (length Γ = length ((zip_with (λ (x : expr → expr) (z : val), x (of_val z))
+          ((λ τ0 : type, App ν (of_val (cast' ℓ τ0 Unknown))) <$> Γ)
+          vs'))) as eq.
+      { rewrite zip_with_length fmap_length. lia. }
+      rewrite -> eq at 1. clear eq. apply LamN_AppWithList_to_vals.
+      rewrite zip_with_fmap_l.
+      apply Forall2_same_length_lookup_2.
+      rewrite zip_with_length. try lia.
+      intros i x x' Hl Hl'.
+      rewrite lookup_zip_with in Hl.
+      assert (lt1 := lookup_lt_Some _ _ _  Hl').
+      destruct (lookup_lt_is_Some_2 Γ i) as [t eq']. lia.
+      simplify_option_eq.
+      eapply (Forall3_lookup_lmr _ _ _ _ i _ _ _ Hs); auto.
+      apply Forall_fmap, Forall_true. by intros t σ x; rewrite /= cast'_closed.
+      by repeat rewrite fmap_length.
+    } iApply Hee'; auto.
+  Qed.
+
+  Lemma open_exprel_superfluous_ctx_r L ℓ Γ e e' (He' : Closed_n (length Γ) e') τ :
+    open_exprel_typed Γ L e e' τ →
+    open_exprel_typed Γ L
+      e
+      (AppWithList (LamN (length Γ) ((App ν (of_val $ cast' ℓ Unknown τ) e')))
+                   (WrapVars ((fun τ => App ν (of_val $ cast' ℓ τ Unknown)) <$> Γ))) τ.
+  Proof.
+    intros Hee'.
+    apply open_exprel_superfluous_ctx_r_help; auto.
+    intros σ. asimpl. by rewrite He' -cast_downwards_rw cast'_closed.
+    by apply open_exprel_superfluous_rtn_r.
+  Qed.
+
+End superfluous_r.
