theories/theorems.v
@@ -1,0 +1,185 @@
+From main.prelude Require Import imports autosubst.
+From main.maps Require Import
+  dyn_embedding.definition linker.definition grad_into_dyn.definition.
+From main.grad_lang Require Import definition types typing contexts labels.
+From main.dyn_lang Require Import definition contexts labels casts.
+From main.logrel Require Import definition adequacy.
+From main.logrel.lemmas Require Import fun_grad_into_dyn fun_dyn_embedding.
+
+Notation dexpr := dyn_lang.definition.expr.
+Notation gexpr := grad_lang.definition.expr.
+
+Notation gctx := grad_lang.contexts.ctx.
+
+Notation dfill_ctx := dyn_lang.contexts.fill_ctx.
+Notation gfill_ctx := grad_lang.contexts.fill_ctx.
+
+Ltac rw_labelrel :=
+    (repeat
+        ((try rewrite /InGradCtx);
+        (try rewrite /InDynExpr);
+        (try rewrite /diagonal);
+        (try rewrite /combine_LabelRel);
+        (try rewrite /elemhood);
+        (try rewrite /join /join_LabelRel_inst /join_LabelRel);
+        (try rewrite /join /join_LabelPred_inst))
+    ).
+
+Ltac le_perm_solver := rw_labelrel; intros ?; set_solver.
+Ltac labelrel_solver := rw_labelrel; set_solver.
+
+Section refined_dyn_emb_criterion.
+
+  Context {ν : label} {Hν : NeverOccurs ν}.
+
+  Definition robust_up_to (L : label → Prop) Γ (e : gexpr) τ : Prop :=
+    ∀ (C : gctx) τ' (HC : typed_ctx C Γ τ [] τ'),
+    (∀ ℓ, rtc step ⟨ gfill_ctx C e ⟩ (Error ℓ) → L ℓ ∨ ℓ ∈ (labels_ctx C)).
+
+  Notation robust := (robust_up_to (fun _ => False)).
+
+  Definition import ℓ Γ τ (e : dexpr) : gexpr :=
+     gfill_ctx (linker ℓ Γ τ) ⌈⌈ e ⌉⌉.
+
+  Lemma rel_ctx_fill_expr {L} (Le Lc : LabelRel) {Γ τ Γ' τ' e e' C C'}
+      (HCC' : ctx_rel_typed Lc C C' Γ τ Γ' τ')
+      (Hee' : open_exprel_typed Γ Le e e' τ)
+      (H : Le ⊔ Lc ⊑ L) :
+    open_exprel_typed Γ' L (fill_ctx C e) (fill_ctx C' e') τ'.
+  Proof.
+    eapply open_exprel_typed_weaken.
+    apply (HCC' (Le ⊔ Lc)). by apply le_permissive_join_r.
+    eapply open_exprel_typed_weaken. apply Hee'.
+    by apply le_permissive_join_l. auto.
+  Qed.
+
+  Theorem general_theorem_lose_import ℓ Γ L (e e' : dexpr) (H : Closed_n (length Γ) e) τ
+    (Hee' : open_exprel_typed Γ L e e' τ)
+    (C : gctx) τ' (HC : typed_ctx C Γ τ [] τ') :
+       ⟨gfill_ctx C (import ℓ Γ τ e)⟩ ≤{L ⊔ (InGradCtx C)}
+          (fill_ctx (trns_ctx C) e').
+  Proof.
+    repeat rewrite trns_fill_ctx.
+    apply (refineL_trans
+              ((InGradCtx C) ⊔ (diagonal ({[ ℓ ]} : listset label)) ⊔ (InDynExpr e))
+              ((InGradCtx C) ⊔ L)
+                (dfill_ctx (trns_ctx C)
+                     (dfill_ctx (trns_ctx (linker ℓ Γ τ)) e))); [le_perm_solver | | ].
+    - (* taking care of dyn embedding *)
+      eapply logrel_adequacy.
+      eapply (rel_ctx_fill_expr (diagonal ({[ℓ]} : listset label) ⊔ (InDynExpr e))). by eapply fundamental_ctx. 2: le_perm_solver.
+      apply linker_compat; auto; try by labelrel_solver.
+        by apply dyn_emb_trns_pres_closed_n.
+        eapply open_exprel_typed_weaken. apply fundamental_l; auto. le_perm_solver.
+    - (* superfluous linker *)
+      eapply logrel_adequacy.
+      eapply (rel_ctx_fill_expr L). by eapply fundamental_ctx. 2: le_perm_solver.
+      apply linker_superfluous_l; auto.
+  Qed.
+
+
+  Theorem refined_dyn_emb_criterion_generalized Γ L (e : dexpr) τ
+    (He : sem_typed_liable_to L Γ e τ) κ : robust_up_to L Γ (import κ Γ τ e) τ.
+  Proof.
+    rewrite /robust_up_to. intros. destruct He as [He Hc].
+    assert (HRef := general_theorem_lose_import κ _ _ _ _ Hc _ He _ _ HC).
+    destruct HRef as [_ Hl]. specialize (Hl ℓ H). destruct Hl as (ℓ' & Hℓ' & _).
+    revert Hℓ'. labelrel_solver.
+  Qed.
+
+  Theorem refined_dyn_emb_criterion Γ (e : dexpr) (H : Closed_n (length Γ) e) τ
+    (He : sem_typed Γ e τ) κ : robust Γ (import κ Γ τ e) τ.
+  Proof. by apply refined_dyn_emb_criterion_generalized. Qed.
+
+
+End refined_dyn_emb_criterion.
+
+Section rrhp_sem_typed.
+
+  Context {ν : label} {Hν : NeverOccurs ν}.
+
+  Theorem general_theorem_gain_import ℓ Γ L (e e' : dexpr) (H : Closed_n (length Γ) e') τ
+    (Hee' : open_exprel_typed Γ L e e' τ)
+    (C : gctx) τ' (HC : typed_ctx C Γ τ [] τ') :
+    RefineL (L ⊔ (InGradCtx C))
+       (fill_ctx (trns_ctx C) e)
+       ⟨gfill_ctx C (import ℓ Γ τ e')⟩.
+  Proof.
+    repeat rewrite trns_fill_ctx.
+    apply (refineL_trans
+              ((InGradCtx C) ⊔ L)
+              ((InGradCtx C) ⊔ (diagonal ({[ ℓ ]} : listset label)) ⊔ (InDynExpr e'))
+                (dfill_ctx (trns_ctx C)
+                     (dfill_ctx (trns_ctx (linker ℓ Γ τ)) e'))); [le_perm_solver | | ].
+    - (* superfluous linker *)
+      eapply logrel_adequacy.
+      eapply (rel_ctx_fill_expr L). by eapply fundamental_ctx. 2: le_perm_solver.
+      apply linker_superfluous_r; auto.
+    - (* taking care of dyn embedding *)
+      eapply logrel_adequacy.
+      eapply (rel_ctx_fill_expr (diagonal ({[ℓ]} : listset label) ⊔ (InDynExpr e'))). by eapply fundamental_ctx. 2: le_perm_solver.
+      apply linker_compat; auto; try by labelrel_solver.
+        by apply dyn_emb_trns_pres_closed_n.
+        eapply open_exprel_typed_weaken. apply fundamental_r; auto. le_perm_solver.
+  Qed.
+
+  Theorem rrhp_import_sem_typed Γ L (e : dexpr) τ (He : sem_typed_liable_to L Γ e τ) :
+   ∀ ℓ (C : gctx) τ' (HC : typed_ctx C Γ τ [] τ'),
+       ⟨gfill_ctx C (import ℓ Γ τ e)⟩
+           ≡{ L ⊔ labels_ctx C }
+       (fill_ctx (trns_ctx C) e).
+  Proof.
+    intros. destruct He as [He Hc]. split.
+    - eapply RefineL_weaken.
+      eapply general_theorem_lose_import; eauto. le_perm_solver.
+    - eapply RefineL_weaken.
+      eapply general_theorem_gain_import; eauto. le_perm_solver.
+  Qed.
+
+
+End rrhp_sem_typed.
+
+Section rrhp_untyped.
+
+  Context {ν : label} {Hν : NeverOccurs ν}.
+
+  Theorem general_theorem_gain_dyn_emb n (e : dexpr) (H : Closed_n n e)
+    (C : gctx) τ (HC : typed_ctx C (replicate n Unknown) Unknown [] τ) :
+    RefineL (InGradCtx C ⊔ InDynExpr e)
+       (fill_ctx (trns_ctx C) e)
+       ⟨gfill_ctx C ⌈⌈ e ⌉⌉⟩.
+  Proof.
+    repeat rewrite trns_fill_ctx.
+    eapply logrel_adequacy.
+    eapply (rel_ctx_fill_expr (InDynExpr e)).
+    by eapply fundamental_ctx. 2: le_perm_solver.
+    eapply open_exprel_typed_weaken. apply fundamental_r; auto. le_perm_solver.
+  Qed.
+
+  Theorem general_theorem_lose_dyn_emb n (e : dexpr) (H : Closed_n n e)
+    (C : gctx) τ (HC : typed_ctx C (replicate n Unknown) Unknown [] τ) :
+    RefineL (InGradCtx C ⊔ InDynExpr e)
+       ⟨gfill_ctx C ⌈⌈ e ⌉⌉⟩
+       (fill_ctx (trns_ctx C) e).
+  Proof.
+    repeat rewrite trns_fill_ctx.
+    eapply logrel_adequacy.
+    eapply (rel_ctx_fill_expr (InDynExpr e)).
+    by eapply fundamental_ctx. 2: le_perm_solver.
+    eapply open_exprel_typed_weaken. apply fundamental_l; auto. le_perm_solver.
+  Qed.
+
+  Theorem rrhp_dyn_emb_untyped n (e : dexpr) (H : Closed_n n e) :
+    ∀ (C : gctx) τ (HC : typed_ctx C (replicate n Unknown) Unknown [] τ),
+       (fill_ctx (trns_ctx C) e)
+           ≡{ (labels_expr e : label → Prop) ⊔ (labels_ctx C) }
+       ⟨gfill_ctx C ⌈⌈ e ⌉⌉⟩.
+  Proof.
+    intros. split.
+    - eapply RefineL_weaken.
+      eapply general_theorem_gain_dyn_emb; eauto. le_perm_solver.
+    - eapply RefineL_weaken.
+      eapply general_theorem_lose_dyn_emb; eauto. le_perm_solver.
+  Qed.
+
+End rrhp_untyped.
